MapFind.v
@@ -1,0 +1,30 @@
+Require Import Coq.FSets.FSetAVL.
+Require Import Coq.FSets.FSetWeakList.
+Require Import Coq.MSets.MSetWeakList.
+Require Import Coq.FSets.FSetFacts.
+Require Import Coq.FSets.FMapAVL.
+Require Import Coq.FSets.FMapFacts.
+
+Require Import Top0.Keys.
+
+Inductive type2 :=
+  | Ty2_Natural : type2
+  | Ty2_Boolean : type2.
+
+Definition tau := type2.
+
+Module ST := FMapAVL.Make (RegionVars).
+Definition Sigma : Type := ST.t tau.
+
+Module STMapP := FMapFacts.Facts ST.
+Module STRaw := ST.Raw.
+Module STProofs := ST.Raw.Proofs.
+
+  
+Definition Functional_Map_Union (stty1 stty2 : Sigma) : Sigma :=
+  let f := fun (k : nat * nat) (v : tau) (m : Sigma) => ST.add k v m
+  in ST.fold f stty1 stty2.
+  
+Axiom Functional_Map_Union_find:
+  forall sttya sttyb (l : ST.key) (t' : tau),
+    ST.find (elt:=tau) l (Functional_Map_Union sttya sttyb) = ST.find (elt:=tau) l sttya.
